Finished L3-L3_eta-L4 proofs entirely, no assumptions remaining except due to WApp_e changes by Randy.

theories/L4_deBruijn/L3_to_L3_eta.v
@@ -1,7 +1,17 @@
 (** Intermediate L3_eta language.
 
   Enforce eta-expanded branches in match, so that the following L3-L4 phase
-  can strip them correctly. *)
+  can strip them correctly. 
+
+  Note that we cannot optimize by not eta-expanding a branch which has already
+  enough lambdas as this would not be a substitutive operation: 
+  translation of terms before or after substitution would only be alpha-beta equivalent,
+  not syntactically equal.
+
+  We hence leave it to later phases to reduce the potentially dummy beta-redexes
+  that are produced here. They would be of the form (\x1 .. xn. t) y1 .. yn where the
+  y's are always variables.
+*)
 
 Require Import Coq.Arith.Arith Coq.NArith.BinNat Coq.Strings.String Coq.Lists.List
         Coq.omega.Omega Coq.Program.Program Coq.micromega.Psatz.
@@ -36,16 +46,11 @@ Section TermTranslation.
      Γ, x1 : τ1, .., xn : τn |- body x1 .. xn : τ
    *)
 
-  Fixpoint eta_expand_aux (n : nat) (t : Term) : Term :=
+  Fixpoint eta_expand (n : nat) (t : Term) : Term :=
     match n with
     | 0%nat => t
-    | S n' =>
-      TLambda nAnon (eta_expand_aux n' (TApp (lift 0 t) (TRel 0)))
+    | S n' => TLambda nAnon (eta_expand n' (TApp (lift 0 t) (TRel 0)))
     end.
-
-  Definition eta_expand n t :=
-    if is_n_lambda n t then t
-    else eta_expand_aux n t.
       
   Eval compute in is_n_lambda 1 (TLambda (nNamed "x") (TRel 0)).
   Eval compute in eta_expand 1 (TLambda (nNamed "x") (TRel 0)).
@@ -57,51 +62,48 @@ Section TermTranslation.
   Eval compute in eta_expand 1 (TLambda (nNamed "x") (TRel 0)).
   Eval compute in eta_expand 2 (TLambda (nNamed "x") (TRel 1)).
   
-  Fixpoint trans (k : nat) (t : Term) : Term :=
+  Fixpoint trans (t : Term) : Term :=
     match t with
     | TWrong str => TWrong str
     | TProof => TProof
     | TRel n => TRel n
-    | TLambda n t => TLambda n (trans (1+k) t)
-    | TLetIn n t u => TLetIn n (trans k t) (trans (1+k) u)
-    | TApp t u => TApp (trans k t) (trans k u)
+    | TLambda n t => TLambda n (trans t)
+    | TLetIn n t u => TLetIn n (trans t) (trans u)
+    | TApp t u => TApp (trans t) (trans u)
     | TConst s => TConst s
     | TConstruct ind c args =>      
-      TConstruct ind c (trans_terms k args)
+      TConstruct ind c (trans_terms args)
     | TCase ind t brs =>
-      TCase ind (trans k t) (trans_brs ind k brs)
+      TCase ind (trans t) (trans_brs ind brs)
     | TFix d n =>
-      let len := L3t.dlength d in
-      let defs' := trans_fixes (len + k) d in
+      let defs' := trans_fixes d in
       TFix defs' n
     end
 
-  with trans_terms (k : nat) (ts : Terms) : Terms :=
+  with trans_terms (ts : Terms) : Terms :=
     match ts with
     | tnil => tnil
-    | tcons t ts => tcons (trans k t) (trans_terms k ts)
+    | tcons t ts => tcons (trans t) (trans_terms ts)
     end
-  with trans_brs (i : inductive) (k : nat) (brs : Brs) : Brs :=
+  with trans_brs (i : inductive) (brs : Brs) : Brs :=
     match brs with
     | bnil => bnil
     | bcons n t brs =>
-      let transt := trans k t in
+      let transt := trans t in
       let etat := eta_expand n transt in
-      bcons n etat (trans_brs i k brs)
+      bcons n etat (trans_brs i brs)
     end
-  with trans_fixes (k : nat) (d : Defs) : Defs :=
+  with trans_fixes (d : Defs) : Defs :=
     match d with
     | dnil => dnil
-    | dcons na t n ds => dcons na (trans k t) n (trans_fixes k ds)
+    | dcons na t n ds => dcons na (trans t) n (trans_fixes ds)
     end.
   
 End TermTranslation.
 
-Require Import L3.term L3.program L3.compile L3.wcbvEval.
-
 Fixpoint transEC (ec:envClass Term) : envClass Term :=
   match ec with
-    | ecTrm t => ecTrm (trans 0 t)
+    | ecTrm t => ecTrm (trans t)
     | ecTyp _ n itp => ecTyp _ n itp
   end.
 
@@ -111,423 +113,16 @@ Fixpoint transEnv (p:environ Term) : environ Term :=
     | cons (nm, ec) q => cons (nm, transEC ec) (transEnv q)
   end.
 
-
-Lemma Lookup_trans_env e nm t : LookupDfn nm e t -> LookupDfn nm (transEnv e) (trans 0 t).
-Proof.
-  red. intros H. red in H.
-  dependent induction H. simpl. constructor.
-  constructor; auto.
-Qed.
-
-Lemma wcbvEval_pres_Crct e t t' :
-  crctTerm e 0 t -> WcbvEval e t t' -> crctTerm e 0 t'.
-Proof.
-  intros.
-  destruct (WcbvEval_pres_Crct e).
-  now apply (H1 t).
-Qed.
-
-Lemma Crct_invrt_Case e n ann mch brs :
-  crctTerm e n (TCase ann mch brs) ->
-  crctTerm e n mch /\ crctBs e n brs /\
-  crctAnnot e ann brs /\
-  (forall i t, bnth i brs = Some t -> crctTerm e n (fst t)).
-Proof.
-  intros.
-  apply Crct_invrt_Case in H. intuition. clear H2.
-  revert H i t H1.
-  induction 1; simpl; intros; try discriminate.
-  destruct i. injection H2 as <-; auto.
-  eapply IHcrctBs; eauto.
-Qed.
-
-Lemma Crct_construct {e : environ Term} {i n args} : crctEnv e ->
-  crctTerm e 0 (TConstruct i n args) ->
-  cnstrArity e i n = Ret (0%nat, tlength args).
-Proof.
-  intros.
-  destruct i.
-  apply Crct_invrt_Construct in H0 as (crctArgs&itypk&Hlook&ip&Hip&ctr&Hctr&Hargs).
-  unfold cnstrArity.
-  destruct Hlook as [Hlook Hne].
-  apply Lookup_lookup in Hlook.
-  unfold lookupTyp. rewrite Hlook. destruct itypk. elim Hne; reflexivity.
-  rewrite Hip, Hctr. unfold ret. repeat f_equal. assumption.
-Qed.
-
-Lemma bnth_trans n t i brs :
-  bnth n brs = Some t -> exists t',
-    bnth n (trans_brs i 0 brs) = Some t' /\
-    fst t' = eta_expand (snd t) (trans 0 (fst t)).
-Proof.
-  revert n t i; induction brs; intros *.
-  simpl; intros. discriminate.
-  
-  simpl. destruct n0. simpl.
-  intros [= <-].
-  eexists; split; eauto.
-  simpl.
-  
-  intros. now eapply IHbrs.
-Qed.
-      
-Arguments raise : simpl never.
-Arguments String.append : simpl never.
-
-Lemma match_annot_n {cnstrs brs n c t} :
-  match_annot cnstrs brs ->
-  exnNth cnstrs n = Ret c ->
-  bnth n brs = Some t -> CnstrArity c = snd t.
-Proof.
-  intros H; revert n c t; induction H; intros; simpl; auto.
-  - discriminate.
-  - destruct n. injection H1; intros ->. injection H2; intros <-.
-    simpl; auto.
-
-    simpl in H1, H2.
-    now specialize (IHmatch_annot _ _ _ H1 H2).
-Qed.
-
-Lemma WcbvEval_mkApp_einv {e f a s} : WcbvEval e (mkApp f a) s ->
-                                      exists s', WcbvEval e f s'.
-Proof.
-  revert f; induction a; simpl; intros.
-  - exists s. intuition. 
-  - specialize (IHa (TApp f t) H).
-    destruct IHa. inv H0.
-    + exists (TLambda nm bod). assumption.
-    + exists (TFix dts m). assumption.
-    + destruct H4; (exists fn'; assumption).
-Qed.
-
-Lemma WcbvEval_is_n_lam e n t t' : is_n_lambda n t = true -> WcbvEval e t t' -> is_n_lambda n t' = true.
-Proof.
-  induction n; simpl; intros Hlam; auto.
-  
-  destruct t; try discriminate.
-  intros. inv H.
-  auto.
-Qed.
-
-Lemma wcbvEval_no_step e s t : WcbvEval e s t -> WcbvEval e t t.
-Proof.
-  apply WcbvEval_no_further.
-Qed.
-Hint Resolve wcbvEval_no_step.
-
-Lemma WcbvEval_mkApp_inner e f s' a s :
-  (WcbvEval e f s' ->
-   WcbvEval e (mkApp s' a) s -> WcbvEval e (mkApp f a) s) /\
-  (WcbvEval e f s' ->
-   WcbvEval e (mkApp f a) s -> WcbvEval e (mkApp s' a) s).
-  
-Proof.
-  revert f s' s; induction a; intros *; split; intros evf evapp; simpl in *.
-  - pose (wcbvEval_no_step _ _ _ evf). rewrite <- (WcbvEval_single_valued w evapp). eauto.
-  - rewrite <- (WcbvEval_single_valued evf evapp). eauto.
-    
-  - simpl in *.
-    destruct (WcbvEval_mkApp_einv evapp) as [s'' evs''].
-    assert(WcbvEval e (TApp f t) s'').
-    { pose (wcbvEval_no_step _ _ _ evf). inv evs''. 
-      + pose proof (WcbvEval_single_valued w H1). subst s'.
-        eapply wAppLam; eassumption.
-      + pose proof (WcbvEval_single_valued w H1). subst s'. 
-        eapply wAppFix; eassumption.
-      + pose proof (WcbvEval_single_valued w H1). subst s'.
-        eapply wAppCong; eassumption. }
-    eapply (proj1 (IHa (TApp f t) s'' s)); eauto.
-    eapply (proj2 (IHa (TApp s' t) s'' s)); eauto.
-
-  - simpl in *.
-    destruct (WcbvEval_mkApp_einv evapp) as [s'' evs''].
-    assert(WcbvEval e (TApp s' t) s'').
-    { inv evs''. 
-      + pose proof (WcbvEval_single_valued evf H1). subst s'.
-        eapply wAppLam; try eassumption. econstructor.
-      + pose proof (WcbvEval_single_valued evf H1). subst s'. 
-        eapply wAppFix; try eassumption. econstructor.
-      + pose proof (WcbvEval_single_valued evf H1). subst s'.
-        eapply wAppCong; try eassumption.
-        apply (proj1 (WcbvEval_no_further e) _ _ H1 ). }
-    eapply (proj1 (IHa _ _ s)). eauto.
-    eapply (proj2 (IHa _ _ s)). eapply evs''. apply evapp.
-Qed.
-
-Lemma instantiate_eta t k n u : WFTrm t 0 -> instantiate t k (eta_expand_aux n u) =
-                                            eta_expand_aux n (instantiate t k u).
-Proof.
-  revert k u; induction n; intros. simpl. auto.
-  simpl. rewrite instantiate_TLambda.
-  f_equal. rewrite IHn; auto.
-  f_equal. rewrite instantiate_TApp_commute.
-  f_equal. rewrite <- (proj1 (instantiate_lift _)); auto. 
-  lia.
-Qed.
-  
-Lemma wcbvEval_eta e t s n : WcbvEval e t s -> exists s', WcbvEval e (eta_expand_aux n t) s'.
-Proof.
-  induction n; intros.
-  simpl.
-  - now exists s.
-  - simpl. eexists. constructor.
-Qed.
-
-Lemma is_n_lambda_eta n t : is_n_lambda n (eta_expand_aux n t) = true.
-Proof.
-  revert t; induction n; intros; trivial.
-  simpl. now rewrite IHn.
-Qed.
-
-Lemma eval_app_terms e f args s :
-  WFTrms args 0 -> WcbvEvals e args args ->
-  WcbvEval e (mkApp f args) s ->
-  WcbvEval e (mkApp (eta_expand (tlength args) f) args) s.
-Proof.
-  intros wfargs nosteps.
-  unfold eta_expand. case_eq (is_n_lambda (tlength args) f). trivial.
-  intros _.
-  revert e f s wfargs nosteps; induction args; intros.
-  { simpl; trivial. }
-  simpl in *; pose proof (WcbvEval_mkApp_einv H).
-  destruct H0 as [s' evft].
-  destruct (wcbvEval_eta _ _ _ (tlength args) evft).
-
-  eapply WcbvEval_mkApp_inner with (s':=x). 
-  - eapply wAppLam with (a1':=t). constructor.
-    now inv nosteps.
-    unfold whBetaStep.
-    rewrite instantiate_eta.
-    rewrite instantiate_TApp_commute.
-    cbn. rewrite (proj1 (instantiate_noLift t)).
-    exact H0. now inv wfargs.
-  - eapply (proj2 (WcbvEval_mkApp_inner _ _ _ _ _)). eauto.
-    eapply IHargs. now inv wfargs. now inv nosteps. eauto.
-Qed.    
-
-Lemma trans_terms_pres_tlength n a : tlength a = tlength (trans_terms n a).
-Proof. induction a; trivial. simpl. now rewrite IHa. Qed.
-
-Lemma trans_mkApp n t u : trans n (mkApp t u) = mkApp (trans n t) (trans_terms n u).
-Proof.
-  revert t; induction u; trivial.
-  simpl. intros. now rewrite IHu. 
-Qed.
-
-Lemma whCase_step e i n args brs cs s :
-  crctEnv e -> crctBs e 0 brs -> crctAnnot e i brs -> crctTerms e 0 args ->
-  cnstrArity e i n = Ret (0%nat, tlength args) ->
-  whCaseStep n args brs = Some cs -> WcbvEval e cs s ->
-  WcbvEvals (transEnv e) (trans_terms 0 args) (trans_terms 0 args) ->
-  WcbvEval (transEnv e) (trans 0 cs) (trans 0 s) ->
-  exists cs',
-    whCaseStep n (trans_terms 0 args) (trans_brs i 0 brs) =
-    Some cs' /\ WcbvEval (transEnv e) cs' (trans 0 s).
-Proof.
-  intros crcte crctds crctann crctargs crctar Hcase Hev evargs IHev.
-  unfold whCaseStep in Hcase.
-  revert Hcase; case_eq (bnth n brs). intros [t arg] Hdn [= <-].
-  unfold whCaseStep.
-  
-  unfold dnthBody in Hdn. case_eq (bnth n brs). intros. rewrite H in Hdn.
-  destruct (bnth_trans _ _ i _ H) as [cs' [Hnth Heq]].
-  unfold dnthBody. rewrite Hnth. destruct cs'. simpl in *.
-  eexists; split; eauto.
-  
-  destruct p. simpl in *.
-  injection Hdn. intros -> ->.
-  assert(tlength args = arg).
-  { unfold crctAnnot in *. destruct i as [nm ndx].
-    destruct crctann as [pack [ityp [Hlook [Hind Hann]]]].
-    unfold cnstrArity in crctar. red in Hlook. destruct Hlook as [Hlook none].
-    apply Lookup_lookup in Hlook. unfold lookupTyp in *. rewrite Hlook in crctar.
-    destruct pack; try discriminate. rewrite Hind in crctar.
-    unfold getCnstr in crctar. case_eq (exnNth (itypCnstrs ityp) n).
-    intros. rewrite H0 in crctar. discriminate.
-    intros; rewrite H0 in crctar.
-    injection crctar. intros.
-    assert (me:=match_annot_n Hann H0 H). simpl in me. congruence. }
-  clear Hnth H .
-
-  clear crctar Hdn.
-  subst t0. simpl in *. rewrite <- H0.
-  rewrite (trans_terms_pres_tlength 0 args).
-  eapply eval_app_terms.
-  eapply (proj1 (proj2 Crct_WFTrm)).
-  (* trans preserves crct *)
-  admit.
-  apply evargs.
-  now rewrite trans_mkApp in IHev.
-
-  intros. rewrite H in Hdn. discriminate.
-
-  intros. discriminate.
-Admitted.
-
-Lemma dnthBody_trans n t i brs :
-  dnthBody n brs = Some t -> 
-    dnthBody n (trans_fixes i brs) = Some (trans i t).
-Proof.
-  revert n t i; induction brs as [ |na t k ds]; intros *.
-  simpl; intros. discriminate.
-  
-  simpl. destruct n. simpl.
-  intros [= <-].
-  eexists; split; eauto.
-  
-  intros. now eapply IHds.
-Qed.
-
-Lemma pre_whFixStep_pres_Crct:
-  forall (dts:Defs) p n a m x,
-    crctDs p (n + dlength dts) dts -> crctTerm p n a ->
-    dnthBody m dts = Some x ->
-    crctTerm p n (pre_whFixStep x dts a).
-Proof.
-  intros.
-  unfold pre_whFixStep.
-  pose (whFixStep_pres_Crct n H m).
-  unfold whFixStep in c. rewrite H1 in c.
-  specialize (c _ eq_refl).
-  constructor. apply c. apply H0.
-Qed.
-
-(** Evaluated constructors have their arguments evaluated *)
-Lemma wcbvEval_construct e mch i n args :
-  crctEnv e -> crctTerm e 0 mch ->
-  WcbvEval e mch (TConstruct i n args) ->
-  WcbvEvals e args args.
-Proof.
-  intros.
-  dependent induction H1.
-  - now eapply WcbvEval_no_further in H1.
-  - eapply IHWcbvEval; eauto. eapply LookupDfn_pres_Crct in H2; eauto.
-  - eapply IHWcbvEval3; eauto.
-    eapply Crct_invrt_App in H0 as [H1 H2].
-    eapply WcbvEval_pres_Crct in H1_; eauto.
-    eapply WcbvEval_pres_Crct in H1_0; eauto.
-    eapply Crct_invrt_Lam in H1_.
-    eapply whBetaStep_pres_Crct; eauto.
-  - eapply IHWcbvEval2; eauto.
-    eapply Crct_invrt_LetIn in H0 as [Hdfn Hbod].
-    eapply WcbvEval_pres_Crct in H1_; eauto.
-    eapply instantiate_pres_Crct; eauto.
-  - eapply IHWcbvEval2; eauto.
-    apply Crct_invrt_App in H0 as [Hfn Harg].
-    eapply WcbvEval_pres_Crct in H1_; eauto.
-    eapply Crct_invrt_Fix in H1_.
-    eapply pre_whFixStep_pres_Crct; eauto.
-  - eapply IHWcbvEval2; eauto.
-    apply Crct_invrt_Case in H0 as (Hmch & Hbrs & Hann & Hts). 
-    eapply WcbvEval_pres_Crct in H1_; eauto.
-    eapply whCaseStep_pres_Crct in H1; eauto.
-    destruct i0; now eapply Crct_invrt_Construct in H1_ as [Hargs0 _].
-Qed.
-
-Theorem translate_correct_subst (e : environ Term) (t t' : Term) :
-  crctEnv e -> crctTerm e 0 t ->
-  WcbvEval e t t' -> 
-  WcbvEval (transEnv e) (trans 0 t) (trans 0 t').
-Proof.
-  assert ((forall t t' : Term,
-  WcbvEval e t t' -> 
-  crctEnv e -> crctTerm e 0 t ->
-  WcbvEval (transEnv e) (trans 0 t) (trans 0 t')) /\
-          (forall t t' : Terms,
-   WcbvEvals e t t' ->
-   crctEnv e -> crctTerms e 0 t ->
-   WcbvEvals (transEnv e) (trans_terms 0 t) (trans_terms 0 t'))).
-  clear; apply WcbvEvalEvals_ind; simpl; auto.
-  - admit.
-(********** this no longer works *****
-  - intros fn arg evprf IHev crcte crctt _ _ _.
-    apply Crct_invrt_App in crctt.
-    constructor. intuition eauto.
- ***********)
-
-(******  - intros i r args args' evargs evtras crcte crctc.
-    destruct i as [ipkg inum]. 
-    apply Crct_invrt_Construct in crctc.
-    intuition.
- *********)
-    
-  - intros nm t s Ht evalt IHt crcte crctt.
-    econstructor; [ | eapply IHt]; eauto.
-    apply Lookup_trans_env; auto.
-    eapply Crct_LookupDfn_Crct; eauto.
-
-  - intros * evfn IHfn evat IHa1 eva1' IHa1' crcte crctc.
-    apply Crct_invrt_App in crctc as [crctfn crcta1].
-    econstructor; eauto.
-
-    assert(trans 0 (whBetaStep bod a1') = whBetaStep (trans 1 bod) (trans 0 a1')).
-    admit.
-    rewrite <- H. apply IHa1'; auto.
-    eapply whBetaStep_pres_Crct.
-    apply wcbvEval_pres_Crct in evfn; auto.
-    now apply Crct_invrt_Lam in evfn.
-    apply wcbvEval_pres_Crct in evat; auto.
-
-  - intros * evdfn IHdfn evbod IHbod crcte crctt.
-    apply Crct_invrt_LetIn in crctt as [crctdn crctbod].
-    econstructor; eauto.
-    forward IHbod; auto. forward IHbod.
-    admit. (* Substitutivity of trans *)
-    apply instantiate_pres_Crct; eauto.
-    eapply WcbvEval_pres_Crct; eauto.
-
-  - intros * evfix IHfix Hfix evapp IHapp crcte crcta.
-    specialize (IHapp crcte).    
-    apply Crct_invrt_App in crcta as [crctfn crctarg].
-    eapply wAppFix with (s := trans 0 s). forward IHfix; auto.
-    apply (dnthBody_trans _ _ (L3t.dlength dts + 0)) in Hfix.
-    apply Hfix.
-    eapply WcbvEval_pres_Crct in evfix; eauto.
-    apply Crct_invrt_Fix in evfix. simpl in evfix.
-    eapply pre_whFixStep_pres_Crct in Hfix; eauto; simpl; eauto.
-    specialize (IHapp Hfix).
-    unfold pre_whFixStep. simpl.
-    admit. (* trans of fixstep *)
-
-  - intros. inversion_Clear H2. eapply wAppCong.
-    + intuition.
-    + destruct o.
-      * left. destruct H2 as [x0 [x1 jx]]. subst. cbn. auto.
-      * right. subst. reflexivity.
-    + intuition.
-
-  - intros * evmch IHmch Hcase evcs IHcs crcte crctc.
-    apply Crct_invrt_Case in crctc as [crctmch [crctbrs [crctann H']]].
-    specialize (IHmch crcte crctmch).
-    pose (whCase_step e i n args brs cs s crcte crctbrs crctann).
-    forward e0. forward e0. specialize (e0 Hcase evcs).
-    forward e0. forward e0. destruct e0 as [cs' [whtrans evtrans]].
-    econstructor; eauto.
-    eapply IHcs; eauto.
-    eapply whCaseStep_pres_Crct in Hcase; eauto.
-    apply wcbvEval_construct in IHmch; eauto.
-    admit. (* Well-formedness preserved by trans *) admit.
-    eapply WcbvEval_pres_Crct in evmch; eauto.
-    now apply Crct_construct in evmch.
-    eapply WcbvEval_pres_Crct in evmch; eauto.
-    destruct i. now eapply Crct_invrt_Construct in evmch as [Hargs _].
-    
-  - intros * evmch IHmch. intros.
-    inv H1.
-    constructor; auto.
-  - intros. apply H; auto.
-Admitted.
-    
 (** start-to-L4 translations **)
 Definition myprogram_Program : program -> Program Term :=
   L3t.program_Program.
 
 Definition translate_program (e : environ L3.compile.Term) (t : L3t.Term) : L3t.Term :=
-  trans 0 t.
+  trans t.
 
 Definition Program_Program (pgm : Program L3t.Term) : Program L3t.Term :=
   let 'mkPgm main env := pgm in
-  {| main := trans 0 main; env := transEnv env |}.
+  {| main := trans main; env := transEnv env |}.
 
 Definition program_L3_eta (pgm:program) : Program L3t.Term :=
   Program_Program (myprogram_Program pgm).
