theories/L4_deBruijn/L3_eta_crct.v
@@ -1,0 +1,695 @@
+(** Intermediate L3_eta language.
+
+  Enforce eta-expanded branches in match, so that the following L3-L4 phase
+  can strip them correctly. *)
+
+Require Import Coq.Arith.Arith Coq.NArith.BinNat Coq.Strings.String Coq.Lists.List
+        Coq.omega.Omega Coq.Program.Program Coq.micromega.Psatz.
+Require Export Common.Common.  (* shared namespace *)
+Require Import L4.expression.
+Require Import L3_to_L3_eta.
+Require Import L3.term L3.program L3.compile L3.wcbvEval.
+
+Set Implicit Arguments.
+Open Scope nat_scope.
+
+(** correctness specification for programs (including local closure) **)
+Inductive crctTerm: environ Term -> nat -> Term -> Prop :=
+| ctRel: forall p n m, crctEnv p -> m < n -> crctTerm p n (TRel m)
+| ctProof: forall p n, crctEnv p -> crctTerm p n TProof
+| ctLam: forall p n nm bod,
+           crctTerm p (S n) bod -> crctTerm p n (TLambda nm bod)
+| ctLetIn: forall p n nm dfn bod,
+             crctTerm p n dfn -> crctTerm p (S n) bod ->
+             crctTerm p n (TLetIn nm dfn bod)
+| ctApp: forall p n fn arg,
+           crctTerm p n fn -> crctTerm p n arg ->
+           crctTerm p n (TApp fn arg)
+| ctConst: forall p n pd nm,
+             crctEnv p -> LookupDfn nm p pd -> crctTerm p n (TConst nm)
+| ctConstructor: forall p n ipkgNm inum cnum args ipkg itp cstr,
+                   LookupTyp ipkgNm p 0 ipkg ->
+                   getInd ipkg inum = Ret itp ->
+                   getCnstr itp cnum = Ret cstr ->
+                   CnstrArity cstr = tlength args ->
+                   crctTerms p n args ->
+                   crctTerm p n (TConstruct (mkInd ipkgNm inum) cnum args)
+| ctCase: forall p n i mch brs,
+    crctTerm p n mch -> crctBs p n brs ->
+    crctAnnot p i brs ->
+    crctTerm p n (TCase i mch brs)
+| ctFix: forall p n ds m,
+           crctDs p (n + dlength ds) ds -> m < dlength ds ->
+           crctTerm p n (TFix ds m)
+(* crctEnvs are closed in both ways *)
+with crctEnv: environ Term -> Prop :=
+| ceNil: crctEnv nil
+| ceTrmCons: forall nm s p,
+    fresh nm p -> crctTerm p 0 s -> crctEnv ((nm,ecTrm s)::p)
+| ceTypCons: forall nm m s p,
+    crctEnv p -> fresh nm p -> crctEnv ((nm,AstCommon.ecTyp Term m s)::p)
+with crctTerms: environ Term -> nat -> Terms -> Prop :=
+| ctsNil: forall p n, crctEnv p -> crctTerms p n tnil
+| ctsCons: forall p n t ts,
+    crctTerm p n t -> crctTerms p n ts -> crctTerms p n (tcons t ts)
+with crctBs: environ Term -> nat -> Brs -> Prop :=
+| cbsNil: forall p n, crctEnv p -> crctBs p n bnil
+| cbsCons: forall p n m t ts,
+    crctTerm p n t -> crctBs p n ts ->
+    (** Eta-expanded branches *)
+    is_n_lambda m t = true ->
+    crctBs p n (bcons m t ts)
+with crctDs: environ Term -> nat -> Defs -> Prop :=
+| cdsNil: forall p n nm bod ix,
+    crctEnv p -> crctTerm p n bod -> isLambda bod ->
+    crctDs p n (dcons nm bod ix dnil)
+| cdsCons: forall p n nm bod ix ds,
+    crctTerm p n bod -> isLambda bod -> crctDs p n ds ->
+    crctDs p n (dcons nm bod ix ds).
+Hint Constructors crctTerm crctTerms crctBs crctDs crctEnv.
+Scheme crct_ind' := Minimality for crctTerm Sort Prop
+  with crcts_ind' := Minimality for crctTerms Sort Prop
+  with crctBs_ind' := Minimality for crctBs Sort Prop
+  with crctDs_ind' := Minimality for crctDs Sort Prop
+  with crctEnv_ind' := Minimality for crctEnv Sort Prop.
+Combined Scheme crctCrctsCrctBsDsEnv_ind from
+         crct_ind', crcts_ind', crctBs_ind', crctDs_ind', crctEnv_ind'.
+
+Lemma crctDs_nonNil:
+  forall p n ds, crctDs p n ds -> dlength ds > 0.
+Proof.
+  induction 1; cbn; intuition.
+Qed.
+
+Lemma Crct_WFTrm:
+  (forall p n t, crctTerm p n t -> WFTrm t n) /\
+  (forall p n ts, crctTerms p n ts -> WFTrms ts n) /\
+  (forall p n bs, crctBs p n bs -> WFTrmBs bs n) /\
+  (forall p n (ds:Defs), crctDs p n ds -> WFTrmDs ds n) /\
+  (forall p, crctEnv p -> True).
+Proof.
+  apply crctCrctsCrctBsDsEnv_ind; intros; auto.
+Qed.
+  
+Lemma Crct_CrctEnv:
+  (forall p n t, crctTerm p n t -> crctEnv p) /\
+  (forall p n ts, crctTerms p n ts -> crctEnv p) /\
+  (forall p n bs, crctBs p n bs -> crctEnv p) /\
+  (forall p n (ds:Defs), crctDs p n ds -> crctEnv p) /\
+  (forall (p:environ Term), crctEnv p -> True).
+Proof.
+  apply crctCrctsCrctBsDsEnv_ind; intros; intuition.
+Qed.
+
+Lemma Crct_up:
+  (forall p n t, crctTerm p n t -> crctTerm p (S n) t) /\
+  (forall p n ts, crctTerms p n ts -> crctTerms p (S n) ts) /\
+  (forall p n bs, crctBs p n bs -> crctBs p (S n) bs) /\
+  (forall p n (ds:Defs), crctDs p n ds -> crctDs p (S n) ds) /\
+  (forall p, crctEnv p -> True). 
+Proof.
+  apply crctCrctsCrctBsDsEnv_ind; intros;
+    try (solve [constructor; assumption]).
+  - apply ctRel; try assumption. omega.
+  - eapply ctConst; eassumption.
+  - eapply ctConstructor; try eassumption.
+Qed.
+
+Lemma CrctDs_Up:
+  forall n p ds, crctDs p n ds -> forall m, n <= m -> crctDs p m ds.
+Proof.
+  intros n p ds h. induction 1. assumption.
+  apply (proj1 (proj2 (proj2 (proj2 Crct_up)))). assumption.
+Qed.
+
+Lemma Crct_UP:
+  forall n p t, crctTerm p n t -> forall m, n <= m -> crctTerm p m t.
+Proof.
+  intros n p t h. induction 1. assumption. apply Crct_up. assumption.
+Qed.
+
+Lemma Crct_Up:
+  forall n p t, crctTerm p 0 t -> crctTerm p n t.
+Proof.
+  intros. eapply Crct_UP. eassumption. omega.
+Qed.
+Hint Resolve Crct_Up Crct_UP.
+
+Lemma Crct_fresh_Pocc:
+  (forall p n t, crctTerm p n t -> forall nm, fresh nm p -> ~ PoccTrm nm t) /\
+  (forall p n ts, crctTerms p n ts ->
+                  forall nm, fresh nm p -> ~ PoccTrms nm ts) /\
+  (forall p n bs, crctBs p n bs ->
+                  forall nm, fresh nm p -> ~ PoccBrs nm bs) /\
+  (forall p n (ds:Defs), crctDs p n ds ->
+                         forall nm, fresh nm p -> ~ PoccDefs nm ds) /\
+  (forall (p:environ Term), crctEnv p -> True).
+Proof.
+  apply crctCrctsCrctBsDsEnv_ind; intros; auto; intros j; auto;
+    inversion_Clear j;
+  try (specialize (H2 _ H3); contradiction);
+  try (specialize (H2 _ H5); contradiction);
+  try (specialize (H5 _ H6); contradiction);
+  try (specialize (H0 _ H3); contradiction);
+  try (specialize (H0 _ H1); contradiction);
+  try (specialize (H0 _ H6); contradiction);
+  try (specialize (H0 _ H4); contradiction);
+  try (specialize (H1 _ H4); contradiction);
+  try (specialize (H1 _ H5); contradiction);
+  try (specialize (H3 _ H4); contradiction);
+  try (specialize (H3 _ H5); contradiction);
+  try (specialize (H3 _ H6); contradiction);
+  try (specialize (H4 _ H5); contradiction).
+  - unfold LookupDfn in H1. elim (Lookup_fresh_neq H1 H2). reflexivity.
+  - unfold LookupTyp in H. destruct H.
+    elim (Lookup_fresh_neq H H5). reflexivity.
+  - specialize (H2 _ H4). contradiction.
+  - destruct H3 as (pack&ityp&Hlook&_).
+    unfold LookupTyp in Hlook. destruct Hlook.
+    elim (Lookup_fresh_neq H3 H4). reflexivity.
+  - specialize (H0 _ H2). contradiction.
+  - specialize (H2 _ H4). contradiction.
+  - specialize (H2 _ H4). contradiction.
+  - inversion H6. 
+Qed.
+
+Lemma Crct_weaken:
+  (forall p n t, crctTerm p n t -> 
+                 forall nm s, fresh nm p -> crctTerm p 0 s ->
+                              crctTerm ((nm,ecTrm s)::p) n t) /\
+  (forall p n ts, crctTerms p n ts -> 
+                  forall nm s, fresh nm p -> crctTerm p 0 s ->
+                               crctTerms ((nm,ecTrm s)::p) n ts) /\
+  (forall p n bs, crctBs p n bs -> 
+                  forall nm s, fresh nm p -> crctTerm p 0 s ->
+                               crctBs ((nm,ecTrm s)::p) n bs) /\
+  (forall p n ds, crctDs p n ds -> 
+                  forall nm s, fresh nm p -> crctTerm p 0 s ->
+                               crctDs ((nm,ecTrm s)::p) n ds) /\
+  (forall p, crctEnv p -> True).
+Proof.
+  apply crctCrctsCrctBsDsEnv_ind; intros;
+  try (solve[repeat econstructor; intuition]);
+  try (econstructor; intuition); try eassumption.
+  - unfold LookupDfn in *. constructor.
+    apply neq_sym. apply (Lookup_fresh_neq H1 H2). eassumption.
+  - destruct H. unfold LookupTyp. split; try eassumption.
+    constructor; try eassumption.
+    apply neq_sym. eapply Lookup_fresh_neq; eassumption.
+  - red. red in H3. destruct i. destruct H3 as [pack [ityp0 [Hlook [Hget Hann]]]].
+    exists pack. exists ityp0. intuition.
+    destruct Hlook. split; auto. constructor; auto.
+    apply neq_sym. eapply Lookup_fresh_neq; eassumption.
+Qed.
+
+Lemma Crct_weaken_Typ:
+  (forall p n t, crctTerm p n t -> 
+                 forall nm s m, fresh nm p ->
+                              crctTerm ((nm,ecTyp Term m s)::p) n t) /\
+  (forall p n ts, crctTerms p n ts -> 
+                  forall nm s m, fresh nm p ->
+                               crctTerms ((nm,ecTyp Term m s)::p) n ts) /\
+  (forall p n ts, crctBs p n ts -> 
+                  forall nm s m, fresh nm p ->
+                               crctBs ((nm,ecTyp Term m s)::p) n ts) /\
+  (forall p n ds, crctDs p n ds -> 
+                  forall nm s m, fresh nm p ->
+                               crctDs ((nm,ecTyp Term m s)::p) n ds) /\
+  (forall p, crctEnv p -> True).
+Proof.
+  apply crctCrctsCrctBsDsEnv_ind; intros;
+  try (solve[repeat econstructor; intuition]);
+  try (econstructor; intuition); try eassumption.
+  - unfold LookupDfn in *. constructor.
+    apply neq_sym. apply (Lookup_fresh_neq H1 H2). eassumption.
+  - unfold LookupTyp in *. destruct H. split; try eassumption.
+    constructor; try eassumption.
+    apply neq_sym. apply (Lookup_fresh_neq H). assumption.
+  - red. red in H3. destruct i. destruct H3 as [pack [ityp0 [Hlook [Hget Hann]]]].
+    exists pack. exists ityp0. intuition.
+    destruct Hlook. split; auto. constructor; auto.
+    apply neq_sym. eapply Lookup_fresh_neq; eassumption.
+Qed.
+
+Lemma Crct_strengthen:
+  (forall pp n s, crctTerm pp n s -> forall nm ec p, pp = (nm,ec)::p ->
+                 ~ PoccTrm nm s -> crctTerm p n s) /\
+  (forall pp n ss, crctTerms pp n ss -> forall nm ec p, pp = (nm,ec)::p ->
+                 ~ PoccTrms nm ss -> crctTerms p n ss) /\
+  (forall pp n ss, crctBs pp n ss -> forall nm ec p, pp = (nm,ec)::p ->
+                 ~ PoccBrs nm ss -> crctBs p n ss) /\
+  (forall pp n ds, crctDs pp n ds -> forall nm ec p, pp = (nm,ec)::p ->
+                 ~ PoccDefs nm ds -> crctDs p n ds) /\
+  (forall (pp:environ Term), crctEnv pp -> crctEnv (List.tl pp)).
+Proof.
+  apply crctCrctsCrctBsDsEnv_ind; intros; subst;
+    try (econstructor; eassumption);
+    try (constructor; try eassumption; inversion_Clear H; assumption).
+  - constructor. eapply H0. reflexivity. intros h. elim H2.
+    constructor. assumption.
+   - constructor. eapply H0. reflexivity.
+    + intros h. elim H4. apply PoLetInDfn. assumption.
+    + eapply H2. reflexivity. intros h. elim H4. eapply PoLetInBod.
+      assumption.                                                   
+  - constructor; try assumption. eapply H0. reflexivity.
+    + intros h. elim H4. eapply PoAppL. assumption.
+    + eapply H2. reflexivity. intros h. elim H4. apply PoAppA. assumption.
+  - econstructor. exact H0. unfold LookupDfn in *.
+    inversion_Clear H1.
+    + elim H3. constructor.
+    + eassumption.
+  - econstructor; try eassumption.
+    + unfold LookupTyp in *. split; intuition.
+      eapply Lookup_strengthen. eassumption. reflexivity.
+      inversion_Clear H5.
+      * elim H6. constructor.
+      * assumption.
+    + eapply H4. reflexivity. intros h. elim H6. apply PoCnstrA.
+      assumption.
+  - econstructor; try eassumption.
+    + eapply H0. reflexivity. intros h. elim H5. constructor. assumption.
+    + eapply H2. reflexivity. intros h. elim H5.
+      apply PoCaseR. assumption.
+    + destruct i. destruct H3 as (pack&ityp&Hlook&Hget&Hann).
+      exists pack, ityp. split; auto.
+      destruct Hlook as [Hlook Hnil]. split; auto.
+      inversion Hlook; subst. elim H5. apply PoCaseAnn. assumption.
+  - econstructor; try eassumption. eapply H0. reflexivity. intros h.
+    elim H3. constructor. assumption.
+  - constructor.
+    + eapply H0. reflexivity. intros h. elim H4. constructor. assumption.
+    + eapply H2. reflexivity. intros h. elim H4. apply PoTtl. assumption.
+  - constructor; auto.
+    + eapply H0. reflexivity. intros h. elim H5. constructor. assumption.
+    + eapply H2. reflexivity. intros h. elim H5. apply PoBtl. assumption.
+  - constructor; try assumption.
+    + eapply H2. reflexivity. intros h. elim H5. constructor. assumption.
+  - constructor; try assumption.
+    + eapply H0. reflexivity. intros h. elim H5. constructor. assumption. 
+    + eapply H3. reflexivity. intros h. elim H5. constructor.
+      destruct (notPoccDefs H5). contradiction.
+  - cbn. eapply (proj1 Crct_CrctEnv). eassumption.
+  - cbn. assumption.
+Qed.
+
+Lemma TWrong_not_Crct:
+  forall p n s, ~ crctTerm p n (TWrong s).
+Proof.
+  induction p; intros; intros h.
+  - inversion h.
+  - eelim IHp. destruct a. eapply (proj1 Crct_strengthen _ _ _ h).
+    + reflexivity.
+    + intros j. inversion j.
+Qed.
+
+(** Crct inversions **)
+
+Lemma LookupDfn_pres_Crct:
+  forall p, crctEnv p -> forall nm u, LookupDfn nm p u ->
+                                      forall m, crctTerm p m u.
+Proof.
+  induction p; intros; unfold LookupDfn in *.
+  - inversion H0.
+  - inversion_Clear H0. inversion_Clear H.
+    + apply (proj1 Crct_weaken); try assumption. apply Crct_Up. assumption.
+    + inversion_Clear H. apply (proj1 Crct_weaken); try assumption.
+      * eapply IHp. apply (proj1 Crct_CrctEnv p _ _ H5). eassumption.
+      * apply (proj1 Crct_weaken_Typ); try assumption.
+        eapply IHp; try eassumption.
+Qed.
+  
+  
+Lemma Crct_invrt_Rel:
+  forall p n m, crctTerm p n (TRel m) -> m < n.
+Proof.
+  intros. inversion_Clear H. assumption.
+Qed.
+
+Lemma pre_Crct_LookupDfn_Crct:
+  (forall p n t, crctTerm p n t ->
+                 forall nm t, LookupDfn nm p t -> crctTerm p 0 t) /\
+  (forall p n ts, crctTerms p n ts ->
+                  forall nm t, LookupDfn nm p t -> crctTerm p 0 t) /\
+  (forall p n bs, crctBs p n bs ->
+                  forall nm t, LookupDfn nm p t -> crctTerm p 0 t) /\
+  (forall p n (ds:Defs), crctDs p n ds ->
+                         forall nm t, LookupDfn nm p t -> crctTerm p 0 t) /\
+  (forall p, crctEnv p -> forall nm t, LookupDfn nm p t -> crctTerm p 0 t).
+Proof.
+  apply crctCrctsCrctBsDsEnv_ind; intros; unfold LookupDfn in *;
+  try (eapply H0; eassumption); try (eapply H1; eassumption).
+  - eapply H4; eassumption.          
+  - inversion H.
+  - inversion_Clear H2.
+    + apply Crct_weaken; assumption.
+    + apply Crct_weaken; try assumption. eapply H1. eassumption.
+  - inversion_Clear H2.
+    + apply Crct_weaken_Typ; try assumption. eapply H0. eassumption.
+Qed.
+
+
+Lemma Crct_invrt_:
+  forall (ev:environ Term), crctEnv ev ->
+  forall nm s p, ev = (nm, ecTrm s)::p -> crctTerm p 0 s.
+Proof.
+  induction 1; intros; subst;
+    try (inversion_Clear H; assumption);
+    try (eapply IHcrctTerm; reflexivity);
+    try (eapply IHcrctTerm1; reflexivity).
+  - myInjection H1. assumption.
+  - discriminate.
+Qed.
+
+Lemma Crct_LookupDfn_Crct:
+  forall p, crctEnv p -> forall nm t, LookupDfn nm p t -> crctTerm p 0 t.
+Proof.
+  intros. eapply pre_Crct_LookupDfn_Crct; eassumption.
+Qed.
+
+Lemma Crct_invrt_Const:
+  forall p n const, crctTerm p n const ->
+  forall nm, const = TConst nm ->
+       exists pd, (LookupDfn nm p pd /\ crctTerm p 0 pd).
+Proof.
+  induction 1; intros; try discriminate. myInjection H1. 
+  pose proof (Crct_LookupDfn_Crct H H0). exists pd. intuition.
+Qed.
+
+Lemma Crct_invrt_Lam:
+  forall p n nm bod, crctTerm p n (TLambda nm bod) -> crctTerm p (S n) bod.
+Proof.
+  intros. inversion_Clear H. assumption.
+Qed.
+
+Lemma Crct_invrt_LetIn:
+  forall p n nm dfn bod, crctTerm p n (TLetIn nm dfn bod) ->
+     crctTerm p n dfn /\ crctTerm p (S n) bod.
+Proof.
+   intros. inversion_Clear H. intuition.
+Qed.
+
+Lemma Crct_invrt_App:
+  forall p n fn arg,
+    crctTerm p n (TApp fn arg) -> crctTerm p n fn /\ crctTerm p n arg.
+Proof.
+   intros. inversion_Clear H. intuition.
+Qed.
+
+Lemma Crct_invrt_Case:
+  forall p n i s us,
+    crctTerm p n (TCase i s us) -> crctTerm p n s /\ crctBs p n us /\ crctAnnot p i us.
+Proof.
+   intros. inversion_Clear H. intuition.
+Qed.
+
+Lemma Crct_invrt_Fix:
+  forall p n ds m, crctTerm p n (TFix ds m) ->
+                   crctDs p (n + dlength ds) ds.
+Proof.
+   intros. inversion_Clear H. intuition.
+Qed.
+
+Lemma Crct_invrt_Construct:
+  forall p n ipkgNm inum cnum args,
+    crctTerm p n (TConstruct (mkInd ipkgNm inum) cnum args) ->
+    crctTerms p n args /\
+    exists itypk,
+      LookupTyp ipkgNm p 0 itypk /\
+      exists (ip:ityp), getInd itypk inum = Ret ip /\
+                        exists (ctr:Cnstr), getCnstr ip cnum = Ret ctr /\
+                                            CnstrArity ctr = tlength args.
+Proof.
+  intros. inversion_Clear H. intuition. exists ipkg. intuition.
+  exists itp. intuition. exists cstr. intuition.
+Qed.
+
+Lemma pre_CrctDs_invrt:
+  forall m dts x, dnth m dts = Some x ->
+     forall p n, crctDs p n dts ->
+                 crctTerm p n (dbody _ x).
+Proof.
+    intros m dts. functional induction (dnth m dts); intros.
+  - discriminate.
+  - myInjection H. cbn. inversion_Clear H0; try assumption.
+  - specialize (IHo _ H). inversion_Clear H0.
+    + discriminate.
+    + eapply IHo. assumption.
+Qed.
+
+Lemma CrctDs_invrt:
+  forall m dts x, dnthBody m dts = Some x ->
+    forall p n, crctDs p n dts -> crctTerm p n x.
+Proof.
+  intros. functional induction (dnthBody m dts).
+  - discriminate.
+  - myInjection H. inversion_Clear H0; try assumption.
+  - inversion_Clear H0.
+    + inversion H.
+    + intuition.
+Qed.
+
+Lemma CrctBs_invrt:
+  forall n p dts, crctBs p n dts -> 
+    forall m x ix, bnth m dts = Some (x, ix) -> crctTerm p n x /\ is_n_lambda ix x = true.
+Proof.
+  induction 1; intros.
+  - inversion H0.
+  - destruct m0.
+    + cbn in H2. myInjection H2. split; assumption.
+    + eapply IHcrctBs. cbn in H1. eassumption.
+Qed.
+
+Lemma Crcts_append:
+  forall p n ts, crctTerms p n ts ->
+  forall us, crctTerms p n us -> crctTerms p n (tappend ts us).
+Proof.
+  induction 1; intros us h; simpl.
+  - assumption.
+  - constructor; intuition.
+Qed.
+
+Lemma mkApp_pres_Crct:
+  forall p n args, crctTerms p n args ->
+                   forall fn, crctTerm p n fn ->
+                              crctTerm p n (mkApp fn args).
+Proof.
+  induction 1; intros; cbn.
+  - assumption.
+  - apply IHcrctTerms. constructor; assumption.
+Qed.
+
+Lemma Instantiate_pres_is_n_lambda tin n t t' :
+  Instantiate tin n t t' -> forall k, is_n_lambda k t = true -> is_n_lambda k t' = true.
+Proof.
+  induction 1; destruct k; simpl; intros; try discriminate || reflexivity.
+  now apply IHInstantiate.
+Qed.
+
+Lemma Instantiate_pres_Crct:
+  forall tin, 
+    (forall n bod ins,
+       Instantiate tin n bod ins ->
+       forall m p, n <= m -> crctTerm p (S m) bod -> crctTerm p m tin ->
+                   crctTerm p m ins) /\
+    (forall n bods inss,
+       Instantiates tin n bods inss ->
+       forall m p, n <= m -> crctTerms p (S m) bods -> crctTerm p m tin ->
+                   crctTerms p m inss) /\
+    (forall n bods inss,
+       InstantiateBrs tin n bods inss ->
+       forall m p, n <= m -> crctBs p (S m) bods -> crctTerm p m tin ->
+                   crctBs p m inss) /\
+    (forall n ds ids,
+       InstantiateDefs tin n ds ids ->
+       forall m p, n <= m -> crctDs p (S m) ds -> crctTerm p m tin ->
+                   crctDs p m ids).
+Proof.
+  intros tin.
+  apply InstInstsBrsDefs_ind; intros; trivial;
+  try (inversion_Clear H0; econstructor; eassumption);
+  try (inversion_Clear H1; constructor; try assumption; apply H; assumption).
+  - inversion_Clear H0. constructor. assumption. omega.
+  - apply ctRel.
+    + inversion H0. assumption.
+    + inversion H0. omega.
+  - inversion_Clear H1. constructor; try assumption.
+    apply H; try assumption. omega. apply (proj1 Crct_up). assumption.
+  - inversion_Clear H2. constructor; try assumption.
+    + apply H; assumption.
+    + apply H0. omega. assumption. apply (proj1 Crct_up). assumption.
+  - inversion_Clear H2. econstructor; try eassumption.
+    + apply H; try eassumption.
+    + apply H0; try eassumption.
+  - inversion_Clear H1. econstructor; try eassumption.
+    rewrite H11. erewrite Instantiates_pres_tlength; try eassumption.
+    reflexivity.
+    apply H; try eassumption.
+  - inversion_Clear H2. constructor; try assumption.
+    + apply H; try eassumption.
+    + apply H0; try eassumption.
+    + destruct i as [ind k].
+      destruct H11 as (pack&ityp&Hlook&Hget&Hann).
+      exists pack, ityp; intuition auto.
+      destruct ityp. simpl in *. clear H H0; revert Hann its i1; clear.
+      induction 1; inversion_clear 1; constructor; auto.
+  - pose proof (InstantiateDefs_pres_dlength i) as k.
+    inversion_Clear H1. constructor; try omega. apply H. omega.
+    + replace (S (m0 + dlength id)) with (S m0 + dlength d); try omega.
+      assumption.
+    + eapply Crct_UP. eassumption. omega.
+  - inversion_Clear H2. apply ctsCons; intuition.
+  - inversion_Clear H2. constructor; intuition.
+    eapply Instantiate_pres_is_n_lambda; eassumption.
+  - inversion_Clear H2.
+    + inversion_Clear i0. apply cdsNil. assumption.
+      * apply H; intuition.
+      * eapply Instantiate_pres_isLambda; eassumption.
+    + constructor.
+      * apply H; intuition.
+      * eapply Instantiate_pres_isLambda; eassumption.
+      * apply H0; intuition.
+Qed.
+
+Lemma instantiate_pres_Crct:
+  forall p m bod, crctTerm p (S m) bod -> forall tin, crctTerm p m tin -> 
+                  forall n, n <= m -> crctTerm p m (instantiate tin n bod).
+Proof.
+  intros.
+  refine (proj1 (Instantiate_pres_Crct tin) _ _ _ _ _ _ _ _ _);
+    try eassumption.
+  refine (proj1 (instantiate_Instantiate tin) _ _).
+Qed.
+
+Lemma whBetaStep_pres_Crct:
+  forall p n bod, crctTerm p (S n) bod ->
+                  forall a1, crctTerm p n a1 ->
+                             crctTerm p n (whBetaStep bod a1).
+Proof.
+  intros. unfold whBetaStep. 
+  apply instantiate_pres_Crct; try assumption. omega.
+Qed.
+
+Lemma bnth_pres_Crct:
+  forall p n (brs:Brs), crctBs p n brs ->
+    forall m x ix, bnth m brs = Some (x, ix) -> crctTerm p n x.
+Proof.
+  intros p n brs h m x ix.
+  functional induction (bnth m brs); intros; auto.
+  - discriminate.
+  - myInjection H. inversion h. assumption.
+  - apply IHo; inversion h; assumption.
+Qed.
+
+Lemma whCaseStep_pres_Crct:
+  forall p n ts, crctTerms p n ts -> forall brs, crctBs p n brs ->
+  forall m s, whCaseStep m ts brs = Some s -> crctTerm p n s.
+Proof.
+  intros p n ts h1 brs h2 m s h3. unfold whCaseStep in h3.
+  assert (j: bnth m brs = None \/ (exists t, bnth m brs = Some t)).
+  { destruct (bnth m brs).
+    + right. exists p0. reflexivity.
+    + left. reflexivity. }
+  destruct j.
+  - rewrite H in h3. discriminate.
+  - destruct H as [x jx]. rewrite jx in h3. destruct x as [y0 y1].
+    myInjection h3. apply mkApp_pres_Crct; try assumption.
+    eapply (bnth_pres_Crct h2). eassumption.
+Qed.
+
+Lemma fold_left_pres_Crct:
+  forall (f:Term -> nat -> Term) (ns:list nat) p (a:nat),
+    (forall u m, m >= a -> crctTerm p (S m) u ->
+               forall n, In n ns -> crctTerm p m (f u n)) ->
+    forall t, crctTerm p (a + List.length ns) t ->
+              crctTerm p a (fold_left f ns t).
+Proof.
+  intros f. induction ns; cbn; intros.
+  - replace (a + 0) with a in H0. assumption. omega.
+  - apply IHns.
+    + intros. apply H; try assumption. apply (or_intror H3).
+    + replace (a0 + S (Datatypes.length ns))
+        with (S (a0 + (Datatypes.length ns))) in H0.
+      assert (j: a0 + Datatypes.length ns >= a0). omega.
+      specialize (H t _ j H0).
+      apply H. apply (or_introl eq_refl). omega.
+Qed.
+
+Lemma dnth_crctDs_crctTerm:
+  forall m dts fs, dnth m dts = Some fs ->
+                   forall p n, crctDs p n dts -> crctTerm p n (dbody _ fs).
+Proof.
+  intros m dts fs.
+  functional induction (dnth m dts); intros; try discriminate.
+  - inversion_Clear H0.
+    + myInjection H. cbn. assumption.
+    + myInjection H. cbn. assumption.
+  - inversion_Clear H0.
+    + discriminate.
+    + apply IHo; try assumption.
+Qed.
+
+
+Lemma dnthBody_pres_Crct:
+  forall m dts fs, dnthBody m dts = Some fs ->
+                   forall p n, crctDs p n dts -> crctTerm p n fs.
+Proof.
+  intros m dts fs.
+  functional induction (dnthBody m dts); intros; try discriminate.
+  - myInjection H. inversion_Clear H0; try assumption.
+  - inversion_Clear H0.
+    + inversion H.
+    + intuition.
+Qed.
+
+Lemma whFixStep_pres_Crct:
+  forall (dts:Defs) p n,
+    crctDs p (n + dlength dts) dts ->
+    forall m s, whFixStep dts m = Some s -> crctTerm p n s.
+Proof.
+  unfold whFixStep. intros. case_eq (dnthBody m dts); intros.
+  - assert (j: m < dlength dts).
+    { eapply dnthBody_lt. eassumption. }
+    rewrite H1 in H0. myInjection H0. apply fold_left_pres_Crct. 
+    + intros. apply instantiate_pres_Crct; try omega. assumption.
+      * pose proof (In_list_to_zero _ _ H3) as j0.
+        constructor; try assumption.
+        pose proof (dnthBody_pres_Crct _ H1 H) as k2.
+        eapply CrctDs_Up. eassumption. omega.
+    + rewrite list_to_zero_length.
+      eapply dnthBody_pres_Crct. eassumption.
+      eapply CrctDs_Up. eassumption. omega.
+  - rewrite H1 in H0. discriminate.
+Qed.
+
+Lemma WcbvEval_pres_Crct:
+  forall p,
+    (forall t s, WcbvEval p t s ->
+                 forall m, crctTerm p m t -> crctTerm p m s) /\
+    (forall ts ss, WcbvEvals p ts ss ->
+                   forall m, crctTerms p m ts -> crctTerms p m ss).
+Proof.
+  intros p.
+  apply WcbvEvalEvals_ind; cbn; intros;
+    try (inversion_Clear H; intuition);
+    try (inversion_Clear H0; intuition);
+    try (inversion_Clear H1; intuition).
+  - econstructor; try eassumption; intuition.
+    rewrite H9. eapply WcbvEvals_pres_tlength; try eassumption.
+  - erewrite (@LookupDfn_single_valued Term _ _ _ _ l H5) in H.
+    eapply H. eapply LookupDfn_pres_Crct; try eassumption.
+  - inversion_Clear H2. specialize (H _ H7). specialize (H0 _ H8).
+    eapply H1. eapply whBetaStep_pres_Crct; try eassumption.
+    inversion_clear H. assumption.
+  - eapply H0. apply instantiate_pres_Crct; try eassumption; try omega.
+    apply H. assumption.
+  - specialize (H _ H6). inversion_Clear H. eapply H0.
+    constructor; try assumption.
+    apply fold_left_pres_Crct.
+    + intros. apply instantiate_pres_Crct; try assumption; try omega.
+      constructor. eapply CrctDs_Up. eassumption. omega.
+      eapply In_list_to_zero. assumption.
+    + apply (dnthBody_pres_Crct _ e). eapply CrctDs_Up. eassumption. 
+      rewrite list_to_zero_length. omega.
+  - apply H0. eapply whCaseStep_pres_Crct; try eassumption.
+    specialize (H _ H7). inversion_Clear H. assumption.
+Qed.
