theories/L4_deBruijn/L3_to_L3_eta_correct.v
@@ -1,0 +1,637 @@
+(** Intermediate L3_eta language.
+
+  Enforce eta-expanded branches in match, so that the following L3-L4 phase
+  can strip them correctly. *)
+
+Require Import Coq.Arith.Arith Coq.NArith.BinNat Coq.Strings.String Coq.Lists.List
+        Coq.omega.Omega Coq.Program.Program Coq.micromega.Psatz.
+Require Export Common.Common.  (* shared namespace *)
+Open Scope N_scope.
+Opaque N.add.
+Opaque N.sub.
+Require Import L4.expression.
+Require Import L3_to_L3_eta.
+
+Require Import L3.term L3.program L3.compile L3.wcbvEval.
+Require L3_eta_crct.
+Module L3C := L3_eta_crct.
+
+Lemma Lookup_trans_env e nm t : LookupDfn nm e t -> LookupDfn nm (transEnv e) (trans t).
+Proof.
+  red. intros H. red in H.
+  dependent induction H. simpl. constructor.
+  constructor; auto.
+Qed.
+
+Lemma wcbvEval_pres_Crct e t t' :
+  crctTerm e 0 t -> WcbvEval e t t' -> crctTerm e 0 t'.
+Proof.
+  intros.
+  destruct (WcbvEval_pres_Crct e).
+  now apply (H1 t).
+Qed.
+
+Lemma Crct_invrt_Case e n ann mch brs :
+  crctTerm e n (TCase ann mch brs) ->
+  crctTerm e n mch /\ crctBs e n brs /\
+  crctAnnot e ann brs /\
+  (forall i t, bnth i brs = Some t -> crctTerm e n (fst t)).
+Proof.
+  intros.
+  apply Crct_invrt_Case in H. intuition. clear H2.
+  revert H i t H1.
+  induction 1; simpl; intros; try discriminate.
+  destruct i. injection H2 as <-; auto.
+  eapply IHcrctBs; eauto.
+Qed.
+
+Lemma L3C_Crct_invrt_Case e n ann mch brs :
+  L3C.crctTerm e n (TCase ann mch brs) ->
+  L3C.crctTerm e n mch /\ L3C.crctBs e n brs /\
+  crctAnnot e ann brs /\
+  (forall i t, bnth i brs = Some t ->
+               is_n_lambda (snd t) (fst t) = true /\
+               L3C.crctTerm e n (fst t)).
+Proof.
+  intros.
+  apply L3C.Crct_invrt_Case in H.
+  destruct H as (H&H'&H'').
+  split; [ | split]; auto. split; auto.
+  clear H H''.
+  induction H'; simpl; intros; try discriminate.
+  destruct i. injection H1 as <-; auto.
+  eapply IHH'; eauto.
+Qed.
+
+Lemma L3C_Crct_construct {e : environ Term} {i n args} : L3C.crctEnv e ->
+  L3C.crctTerm e 0 (TConstruct i n args) ->
+  cnstrArity e i n = Ret (0%nat, tlength args).
+Proof.
+  intros.
+  destruct i.
+  apply L3C.Crct_invrt_Construct in H0 as (crctArgs&itypk&Hlook&ip&Hip&ctr&Hctr&Hargs).
+  unfold cnstrArity.
+  destruct Hlook as [Hlook Hne].
+  apply Lookup_lookup in Hlook.
+  unfold lookupTyp. rewrite Hlook. destruct itypk. elim Hne; reflexivity.
+  rewrite Hip, Hctr. unfold ret. repeat f_equal. assumption.
+Qed.
+
+Lemma Crct_construct {e : environ Term} {i n args} :
+  crctEnv e ->
+  crctTerm e 0 (TConstruct i n args) ->
+  cnstrArity e i n = Ret (0%nat, tlength args).
+Proof.
+  intros.
+  destruct i.
+  apply Crct_invrt_Construct in H0 as (crctArgs&itypk&Hlook&ip&Hip&ctr&Hctr&Hargs).
+  unfold cnstrArity.
+  destruct Hlook as [Hlook Hne].
+  apply Lookup_lookup in Hlook.
+  unfold lookupTyp. rewrite Hlook. destruct itypk. elim Hne; reflexivity.
+  rewrite Hip, Hctr. unfold ret. repeat f_equal. assumption.
+Qed.
+
+Lemma bnth_trans n t i brs :
+  bnth n brs = Some t -> exists t',
+    bnth n (trans_brs i brs) = Some t' /\
+    fst t' = eta_expand (snd t) (trans (fst t)).
+Proof.
+  revert n t i; induction brs; intros *.
+  simpl; intros. discriminate.
+  
+  simpl. destruct n0. simpl.
+  intros [= <-].
+  eexists; split; eauto.
+  simpl.
+  
+  intros. now eapply IHbrs.
+Qed.
+      
+Arguments raise : simpl never.
+Arguments String.append : simpl never.
+
+Lemma match_annot_n {cnstrs brs n c t} :
+  match_annot cnstrs brs ->
+  exnNth cnstrs n = Ret c ->
+  bnth n brs = Some t -> CnstrArity c = snd t.
+Proof.
+  intros H; revert n c t; induction H; intros; simpl; auto.
+  - discriminate.
+  - destruct n. injection H1; intros ->. injection H2; intros <-.
+    simpl; auto.
+
+    simpl in H1, H2.
+    now specialize (IHmatch_annot _ _ _ H1 H2).
+Qed.
+
+Lemma WcbvEval_mkApp_einv {e f a s} : WcbvEval e (mkApp f a) s ->
+                                      exists s', WcbvEval e f s'.
+Proof.
+  revert f; induction a; simpl; intros.
+  - exists s. intuition. 
+  - specialize (IHa (TApp f t) H).
+    destruct IHa. inv H0.
+    * now exists (TLambda nm bod).
+    * now exists (TFix dts m).
+    * now exists fn'.
+Qed.
+
+Lemma WcbvEval_is_n_lam e n t t' : is_n_lambda n t = true -> WcbvEval e t t' -> is_n_lambda n t' = true.
+Proof.
+  induction n; simpl; intros Hlam; auto.
+  
+  destruct t; try discriminate.
+  intros. inv H.
+  auto.
+Qed.
+
+Lemma wcbvEval_no_step e s t : WcbvEval e s t -> WcbvEval e t t.
+Proof.
+  apply WcbvEval_no_further.
+Qed.
+Hint Resolve wcbvEval_no_step.
+
+Lemma WcbvEval_mkApp_inner e f s' a s :
+  (WcbvEval e f s' ->
+   WcbvEval e (mkApp s' a) s -> WcbvEval e (mkApp f a) s) /\
+  (WcbvEval e f s' ->
+   WcbvEval e (mkApp f a) s -> WcbvEval e (mkApp s' a) s).
+  
+Proof.
+  revert f s' s; induction a; intros *; split; intros evf evapp; simpl in *.
+  - pose (wcbvEval_no_step _ _ _ evf). rewrite <- (WcbvEval_single_valued w evapp). eauto.
+  - rewrite <- (WcbvEval_single_valued evf evapp). eauto.
+    
+  - simpl in *.
+    destruct (WcbvEval_mkApp_einv evapp) as [s'' evs''].
+    assert(WcbvEval e (TApp f t) s'').
+    { pose (wcbvEval_no_step _ _ _ evf). inv evs''. 
+      pose proof (WcbvEval_single_valued w H1). subst s'.
+      econstructor; eauto.
+      pose proof (WcbvEval_single_valued w H1). subst s'.
+      eapply wAppFix; eauto.
+      pose proof (WcbvEval_single_valued w H1). subst s'.
+      eapply wAppCong; eauto. }
+    eapply (proj1 (IHa (TApp f t) s'' s)); eauto.
+    eapply (proj2 (IHa (TApp s' t) s'' s)); eauto.
+
+  - simpl in *.
+    destruct (WcbvEval_mkApp_einv evapp) as [s'' evs''].
+    assert(WcbvEval e (TApp s' t) s'').
+    { inv evs''. 
+      pose proof (WcbvEval_single_valued evf H1). subst s'.
+      econstructor; eauto.
+      pose proof (WcbvEval_single_valued evf H1). subst s'.
+      eapply wAppFix; eauto.
+      pose proof (WcbvEval_single_valued evf H1). subst s'.
+      eapply wAppCong; eauto. }
+    eapply (proj1 (IHa _ _ s)). eauto.
+    eapply (proj2 (IHa _ _ s)). eapply evs''. apply evapp.
+Qed.
+
+Lemma instantiate_eta t k n u : WFTrm t 0 -> instantiate t k (eta_expand n u) =
+                                            eta_expand n (instantiate t k u).
+Proof.
+  revert k u; induction n; intros. simpl. auto.
+  simpl. rewrite instantiate_TLambda.
+  f_equal. rewrite IHn; auto.
+  f_equal. rewrite instantiate_TApp_commute.
+  f_equal. rewrite <- (proj1 (instantiate_lift _)); auto. 
+  lia.
+Qed.
+  
+Lemma wcbvEval_eta e t s n : WcbvEval e t s -> exists s', WcbvEval e (eta_expand n t) s'.
+Proof.
+  induction n; intros.
+  simpl.
+  - now exists s.
+  - simpl. eexists. constructor.
+Qed.
+
+Lemma is_n_lambda_eta n t : is_n_lambda n (eta_expand n t) = true.
+Proof.
+  revert t; induction n; intros; trivial.
+  simpl. now rewrite IHn.
+Qed.
+
+Lemma is_n_lambda_lift n t : is_n_lambda n t = true -> forall k, is_n_lambda n (lift k t) = true.
+Proof.
+  revert t; induction n; intros; trivial.
+  destruct t; simpl in *; try discriminate.
+  simpl. now apply IHn.
+Qed.
+
+Lemma eval_app_terms e f args s :
+  WFTrms args 0 -> WcbvEvals e args args ->
+  WcbvEval e (mkApp f args) s ->
+  WcbvEval e (mkApp (eta_expand (tlength args) f) args) s.
+Proof.
+  intros wfargs nosteps.
+  revert e f s wfargs nosteps; induction args; intros.
+  { simpl; trivial. }
+  simpl in *; pose proof (WcbvEval_mkApp_einv H).
+  destruct H0 as [s' evft].
+  destruct (wcbvEval_eta _ _ _ (tlength args) evft).
+
+  eapply WcbvEval_mkApp_inner with (s':=x). 
+  - eapply wAppLam with (a1':=t). constructor.
+    now inv nosteps.
+    unfold whBetaStep.
+    rewrite instantiate_eta.
+    rewrite instantiate_TApp_commute.
+    cbn. rewrite (proj1 (instantiate_noLift t)).
+    exact H0. now inv wfargs.
+  - eapply (proj2 (WcbvEval_mkApp_inner _ _ _ _ _)). eauto.
+    eapply IHargs. now inv wfargs. now inv nosteps. eauto.
+Qed. 
+
+Lemma trans_terms_pres_tlength a : tlength a = tlength (trans_terms a).
+Proof. induction a; trivial. simpl. now rewrite IHa. Qed.
+
+Lemma lifts_preserves_tlength n a : tlength a = tlength (lifts n a).
+Proof. induction a; trivial. simpl. now rewrite IHa. Qed.
+
+Lemma liftds_preserves_dlength n a : dlength a = dlength (liftDs n a).
+Proof. induction a; trivial. simpl. now rewrite IHa. Qed.
+
+Lemma liftbs_preserves_blength n a : blength a = blength (liftBs n a).
+Proof. induction a; trivial. simpl. now rewrite IHa. Qed.
+
+Lemma trans_mkApp t u : trans (mkApp t u) = mkApp (trans t) (trans_terms u).
+Proof.
+  revert t; induction u; trivial.
+  simpl. intros. now rewrite IHu. 
+Qed.
+
+Lemma trans_fixes_pres_dlength f : dlength (trans_fixes f) = dlength f.
+Proof. induction f; simpl; auto. Qed.
+
+Lemma instantiate_hom :
+  (forall bod arg n, WFTrm (trans arg) 0 ->
+      trans (instantiate arg n bod) =
+      instantiate (trans arg) n (trans bod)) /\
+  (forall bods arg n, WFTrm (trans arg) 0 ->
+     trans_terms (instantiates arg n bods) =
+     instantiates (trans arg) n (trans_terms bods)) /\
+  (forall bods arg n, WFTrm (trans arg) 0 -> forall i,
+     trans_brs i (instantiateBrs arg n bods) =
+     instantiateBrs (trans arg) n (trans_brs i bods)) /\
+  (forall ds arg n, WFTrm (trans arg) 0 ->
+          trans_fixes (instantiateDefs arg n ds) =
+     instantiateDefs (trans arg) n (trans_fixes ds)).
+Proof.
+  apply TrmTrmsBrsDefs_ind; intros; try (cbn; easy);
+  try (cbn; rewrite H; easy).
+  - cbn. destruct (lt_eq_lt_dec n0 n); cbn.
+    + destruct s.
+      * rewrite (proj1 (nat_compare_lt n0 n)); try omega. reflexivity.
+      * subst. rewrite (proj2 (nat_compare_eq_iff _ _)); trivial. 
+    + rewrite (proj1 (nat_compare_gt n0 n)); try intro; trivial.
+  - cbn. now rewrite H, H0.
+  - cbn. now rewrite H, H0.
+  - rewrite instantiate_TConstruct. simpl. now rewrite H.
+  - rewrite instantiate_TCase. simpl. now rewrite H, H0.
+  - rewrite !instantiate_TFix; simpl. rewrite H; try easy.
+    rewrite !instantiate_TFix; simpl. 
+    now rewrite trans_fixes_pres_dlength. 
+  - repeat (rewrite !instantiates_tcons; simpl). now rewrite <- H, H0.
+  - repeat (rewrite !instantiateBs_bcons; simpl). f_equal.
+    rewrite H by easy. rewrite instantiate_eta; auto.
+    now apply H0.
+  - repeat (rewrite !instantiateDs_dcons; simpl); now rewrite H, H0. 
+Qed.
+
+Lemma trans_instantiate_any  a k :
+  WFTrm (trans a) 0 ->
+  forall b, trans (L3.term.instantiate a k b) =
+            instantiate (trans a) k (trans b).
+Proof.
+  intros. destruct instantiate_hom. now apply H0.
+Qed.
+
+Lemma trans_instantiate_fix x ds arg :
+  WFTrmDs (trans_fixes ds) (dlength ds) ->
+  pre_whFixStep (trans x) (trans_fixes ds) (trans arg) =
+  trans (pre_whFixStep x ds arg).
+Proof.
+  simpl. unfold pre_whFixStep. f_equal.
+  revert x.
+  set(foo:= TFix (trans_fixes ds)).
+  set(bar:= TFix ds).
+  rewrite trans_fixes_pres_dlength. induction (list_to_zero (dlength ds)).
+  simpl. reflexivity.
+  simpl. intros.
+  subst foo. rewrite <- (trans_instantiate_any (TFix ds a)).
+  rewrite IHl. f_equal. auto. simpl. constructor.
+  rewrite trans_fixes_pres_dlength. apply H.
+Qed.
+
+Lemma Lookup_hom:
+  forall p (s:string) ec,
+    Lookup s p ec -> Lookup s (transEnv p) (transEC ec).
+Proof.
+  induction 1; destruct t.
+  - cbn. apply LHit.
+  - cbn. apply LHit.
+  - cbn. apply LMiss; assumption. 
+  - cbn. apply LMiss; assumption. 
+Qed.
+
+Ltac eeasy := eauto 3; easy.
+
+Lemma transEnv_pres_fresh e nm : fresh nm e -> fresh nm (transEnv e).
+Proof.
+  induction 1; constructor; auto.
+Qed.
+
+Lemma Crct_lift :
+  (forall p n t, L3C.crctTerm p n t -> forall k,
+                 L3C.crctTerm p (S n) (lift k t)) /\
+  (forall p n ts, L3C.crctTerms p n ts -> forall k, L3C.crctTerms p (S n) (lifts k ts)) /\
+  (forall p n bs, L3C.crctBs p n bs -> forall k, L3C.crctBs p (S n) (liftBs k bs)) /\
+  (forall p n ds, L3C.crctDs p n ds -> forall k, L3C.crctDs p (S n) (liftDs k ds)) /\
+  (forall e, L3C.crctEnv e -> True).
+Proof.
+  apply L3C.crctCrctsCrctBsDsEnv_ind; intros; simpl lift; auto; try solve [econstructor; eauto 2].
+  - constructor. auto.
+    destruct (Nat.compare_spec m k); subst; omega.
+  - econstructor; try rewrite <- lifts_preserves_tlength; eauto. 
+  - econstructor; eauto.
+    destruct i; destruct H3 as [ityp [pack H3]]. red. intuition. do 2 eexists; intuition eauto.
+    revert H6; clear. induction 1; constructor; eauto.
+  - econstructor; eauto; rewrite <- liftds_preserves_dlength; eauto.
+  - simpl liftBs. econstructor; eauto. now apply is_n_lambda_lift.
+  - simpl. constructor; auto.
+    destruct H3 as (na & body & ->). exists na; eexists; reflexivity.
+  - simpl. constructor; auto.
+    destruct H1 as (na & body & ->). exists na; eexists; reflexivity.
+Qed.    
+
+Lemma crctTerm_eta e n t : L3C.crctTerm e n t ->
+                            forall m, L3C.crctTerm e n (eta_expand m t).
+Proof.
+  intros.
+  revert n t H.
+  induction m; intros; trivial.
+
+  simpl eta_expand. constructor.
+  eapply IHm. constructor. eapply (proj1 Crct_lift e n t H 0%nat).
+  constructor; eauto with arith. now eapply L3C.Crct_CrctEnv in H.
+Qed.
+
+Lemma trans_pres_Crct :
+  (forall p n t, crctTerm p n t -> L3C.crctTerm (transEnv p) n (trans t)) /\
+  (forall p n ts, crctTerms p n ts ->
+                  L3C.crctTerms (transEnv p) n (trans_terms ts)) /\
+  (forall p n bs, crctBs p n bs -> forall i, L3C.crctBs (transEnv p) n (trans_brs i bs)) /\
+  (forall p n (ds:Defs), crctDs p n ds -> L3C.crctDs (transEnv p) n (trans_fixes ds)) /\
+  (forall p, crctEnv p -> L3C.crctEnv (transEnv p)).
+Proof.
+  apply crctCrctsCrctBsDsEnv_ind; intros; simpl; try solve [econstructor; eauto].
+
+  - apply Lookup_hom in H1. econstructor; eauto. 
+  - red in H. destruct H. apply Lookup_hom in H.
+    econstructor; try split; try eeasy.
+    now rewrite <- trans_terms_pres_tlength.
+  - econstructor; eauto. destruct i.
+    red in H3.
+    destruct H3 as (pack&ityp&Hlook&Hip&Hann).
+    exists pack, ityp. intuition try eeasy.
+    destruct Hlook. split; auto. now apply Lookup_hom in H3. 
+    revert Hann. clear; induction 1; simpl; constructor; auto.
+  - econstructor; rewrite trans_fixes_pres_dlength; eauto.
+  - econstructor; auto.
+    clear -H0. induction m.
+    simpl. apply H0.
+    now eapply crctTerm_eta.
+    apply is_n_lambda_eta.
+  - econstructor; eauto.
+    destruct H3 as (na & body & ->).
+    exists na. eexists; simpl; eauto.
+  - econstructor; eauto.
+    destruct H1 as (na & body & ->).
+    exists na. eexists; simpl; eauto.
+  - econstructor; eauto. 
+    now apply transEnv_pres_fresh.
+  - econstructor; eauto. 
+    now apply transEnv_pres_fresh.
+Qed.
+    
+Lemma whCase_step e i n args brs cs s :
+  crctEnv e -> crctBs e 0 brs -> crctAnnot e i brs -> crctTerms e 0 args ->
+  cnstrArity e i n = Ret (0%nat, tlength args) ->
+  whCaseStep n args brs = Some cs -> WcbvEval e cs s ->
+  WcbvEvals (transEnv e) (trans_terms args) (trans_terms args) ->
+  WcbvEval (transEnv e) (trans cs) (trans s) ->
+  exists cs',
+    whCaseStep n (trans_terms args) (trans_brs i brs) =
+    Some cs' /\ WcbvEval (transEnv e) cs' (trans s).
+Proof.
+  intros crcte crctds crctann crctargs crctar Hcase Hev evargs IHev.
+  unfold whCaseStep in Hcase.
+  revert Hcase; case_eq (bnth n brs). intros [t arg] Hdn [= <-].
+  unfold whCaseStep.
+  
+  unfold dnthBody in Hdn. case_eq (bnth n brs). intros. rewrite H in Hdn.
+  destruct (bnth_trans _ _ i _ H) as [cs' [Hnth Heq]].
+  unfold dnthBody. rewrite Hnth. destruct cs'. simpl in *.
+  eexists; split; eauto.
+  
+  destruct p. simpl in *.
+  injection Hdn. intros -> ->.
+  assert(tlength args = arg).
+  { unfold crctAnnot in *. destruct i as [nm ndx].
+    destruct crctann as [pack [ityp [Hlook [Hind Hann]]]].
+    unfold cnstrArity in crctar. red in Hlook. destruct Hlook as [Hlook none].
+    apply Lookup_lookup in Hlook. unfold lookupTyp in *. rewrite Hlook in crctar.
+    destruct pack; try discriminate. rewrite Hind in crctar.
+    unfold getCnstr in crctar. case_eq (exnNth (itypCnstrs ityp) n).
+    intros. rewrite H0 in crctar. discriminate.
+    intros; rewrite H0 in crctar.
+    injection crctar. intros.
+    assert (me:=match_annot_n Hann H0 H). simpl in me. congruence. }
+  clear Hnth H .
+
+  clear crctar Hdn.
+  subst t0. simpl in *. rewrite <- H0.
+  rewrite (trans_terms_pres_tlength args).
+  eapply eval_app_terms.
+  eapply (proj1 (proj2 L3C.Crct_WFTrm)).
+  (* trans preserves crct *)
+  apply trans_pres_Crct. eassumption.
+  apply evargs.
+  now rewrite trans_mkApp in IHev.
+
+  intros. rewrite H in Hdn. discriminate.
+
+  intros. discriminate.
+Qed.
+
+Lemma dnthBody_trans n t brs :
+  dnthBody n brs = Some t -> 
+    dnthBody n (trans_fixes brs) = Some (trans t).
+Proof.
+  revert n t; induction brs as [ |na t k ds]; intros *.
+  simpl; intros. discriminate.
+  
+  simpl. destruct n. simpl.
+  intros [= <-].
+  eexists; split; eauto.
+  
+  intros. now eapply IHds.
+Qed.
+
+Lemma pre_whFixStep_pres_Crct:
+  forall (dts:Defs) p n a m x,
+    crctDs p (n + dlength dts) dts -> crctTerm p n a ->
+    dnthBody m dts = Some x ->
+    crctTerm p n (pre_whFixStep x dts a).
+Proof.
+  intros.
+  unfold pre_whFixStep.
+  pose (whFixStep_pres_Crct n H m).
+  unfold whFixStep in c. rewrite H1 in c.
+  specialize (c _ eq_refl).
+  constructor. apply c. apply H0.
+Qed.
+
+Lemma L3C_pre_whFixStep_pres_Crct:
+  forall (dts:Defs) p n a m x,
+    L3C.crctDs p (n + dlength dts) dts -> L3C.crctTerm p n a ->
+    dnthBody m dts = Some x ->
+    L3C.crctTerm p n (pre_whFixStep x dts a).
+Proof.
+  intros.
+  unfold pre_whFixStep.
+  pose (L3C.whFixStep_pres_Crct n H m).
+  unfold whFixStep in c. rewrite H1 in c.
+  specialize (c _ eq_refl).
+  constructor. apply c. apply H0.
+Qed.
+
+(** Evaluated constructors have their arguments evaluated *)
+
+Lemma trans_wcbvEval_construct e mch i n args :
+  L3C.crctEnv e -> L3C.crctTerm e 0 mch ->
+  WcbvEval e mch (TConstruct i n args) ->
+  WcbvEvals e args args.
+Proof.
+  intros.
+  dependent induction H1.
+  - now eapply WcbvEval_no_further in H1.
+  - eapply IHWcbvEval; eauto. eapply L3C.LookupDfn_pres_Crct in H2; eauto.
+  - eapply IHWcbvEval3; eauto.
+    eapply L3C.Crct_invrt_App in H0 as [H1 H2].
+    eapply L3C.WcbvEval_pres_Crct in H1_; eauto 2.
+    eapply L3C.WcbvEval_pres_Crct in H1_0; eauto 2.
+    eapply L3C.Crct_invrt_Lam in H1_.
+    eapply L3C.whBetaStep_pres_Crct; eauto.
+  - eapply IHWcbvEval2; eauto.
+    eapply L3C.Crct_invrt_LetIn in H0 as [Hdfn Hbod].
+    eapply L3C.WcbvEval_pres_Crct in H1_; eauto.
+    eapply L3C.instantiate_pres_Crct; eauto.
+  - eapply IHWcbvEval2; eauto.
+    apply L3C.Crct_invrt_App in H0 as [Hfn Harg].
+    eapply L3C.WcbvEval_pres_Crct in H1_; eauto.
+    eapply L3C.Crct_invrt_Fix in H1_.
+    eapply L3C_pre_whFixStep_pres_Crct; eauto.
+  - eapply IHWcbvEval2; eauto.
+    apply L3C_Crct_invrt_Case in H0 as (Hmch & Hbrs & Hann & Hts). 
+    eapply L3C.WcbvEval_pres_Crct in H1_; eauto.
+    eapply L3C.whCaseStep_pres_Crct in H1; eauto.
+    destruct i0; now eapply L3C.Crct_invrt_Construct in H1_ as [Hargs0 _].
+Qed.
+
+Theorem translate_correct_subst (e : environ Term) (t t' : Term) :
+  crctEnv e -> crctTerm e 0 t ->
+  WcbvEval e t t' -> 
+  WcbvEval (transEnv e) (trans t) (trans t').
+Proof.
+  assert ((forall t t' : Term,
+  WcbvEval e t t' -> 
+  crctEnv e -> crctTerm e 0 t ->
+  WcbvEval (transEnv e) (trans t) (trans t')) /\
+          (forall t t' : Terms,
+   WcbvEvals e t t' ->
+   crctEnv e -> crctTerms e 0 t ->
+   WcbvEvals (transEnv e) (trans_terms t) (trans_terms t'))).
+  clear; apply WcbvEvalEvals_ind; simpl; auto.
+
+  - intros i r args args' evargs evtras crcte crctc.
+    destruct i as [ipkg inum]. 
+    apply Crct_invrt_Construct in crctc.
+    intuition.
+
+  - intros nm t s Ht evalt IHt crcte crctt.
+    econstructor; [ | eapply IHt]; eauto.
+    apply Lookup_trans_env; auto.
+    eapply Crct_LookupDfn_Crct; eauto.
+
+  - intros * evfn IHfn evat IHa1 eva1' IHa1' crcte crctc.
+    apply Crct_invrt_App in crctc as [crctfn crcta1].
+    econstructor; eauto 2.
+
+    assert(trans (whBetaStep bod a1') = whBetaStep (trans bod) (trans a1')).
+    unfold whBetaStep. erewrite trans_instantiate_any; eauto.
+    + eapply L3C.Crct_WFTrm. apply trans_pres_Crct. 
+      eapply wcbvEval_pres_Crct; eauto.
+    + rewrite <- H. apply IHa1'; auto.
+      eapply whBetaStep_pres_Crct.
+      apply wcbvEval_pres_Crct in evfn; auto.
+      now apply Crct_invrt_Lam in evfn.
+      apply wcbvEval_pres_Crct in evat; auto.
+
+  - intros * evdfn IHdfn evbod IHbod crcte crctt.
+    apply Crct_invrt_LetIn in crctt as [crctdn crctbod].
+    econstructor; eauto 3.
+    forward IHbod; auto. forward IHbod.
+    erewrite <- trans_instantiate_any; eauto. 
+    { eapply L3C.Crct_WFTrm. eapply trans_pres_Crct.
+      eapply wcbvEval_pres_Crct in evdfn; eauto. }
+    apply instantiate_pres_Crct; eauto.
+    eapply WcbvEval_pres_Crct; eauto.
+
+  - intros * evfix IHfix Hfix evapp IHapp crcte crcta.
+    specialize (IHapp crcte).
+    apply Crct_invrt_App in crcta as [crctfn crctarg].
+    eapply wAppFix with (s := trans s). forward IHfix; auto.
+    apply (dnthBody_trans _ _) in Hfix.
+    apply Hfix.
+    eapply WcbvEval_pres_Crct in evfix; eauto.
+    apply Crct_invrt_Fix in evfix. simpl in evfix.
+    eapply pre_whFixStep_pres_Crct in Hfix; eauto; simpl; eauto.
+    specialize (IHapp Hfix).
+    rewrite trans_instantiate_fix. apply IHapp.
+    eapply L3C.Crct_WFTrm.
+    eapply trans_pres_Crct; eauto.
+
+  - intros fn arg evprf IHev crcte crctt.
+    intros.
+    apply Crct_invrt_App in H1.
+    constructor; intuition eauto. left.
+    destruct H1 as [fn' [arg' ->]]. do 2 eexists; reflexivity.
+    right; subst arg. simpl. reflexivity.
+
+  - intros * evmch IHmch Hcase evcs IHcs crcte crctc.
+    apply Crct_invrt_Case in crctc as [crctmch [crctbrs [crctann H']]].
+    specialize (IHmch crcte crctmch).
+    pose (whCase_step e i n args brs cs s crcte crctbrs crctann).
+    forward e0. forward e0. specialize (e0 Hcase evcs).
+    forward e0. forward e0. destruct e0 as [cs' [whtrans evtrans]].
+    econstructor; eauto.
+    eapply IHcs; eauto.
+    eapply whCaseStep_pres_Crct in Hcase; eauto.
+    apply trans_wcbvEval_construct in IHmch; eauto;
+    eapply trans_pres_Crct; eauto.
+    eapply WcbvEval_pres_Crct in evmch; eauto.
+    now apply Crct_construct in evmch.
+    eapply WcbvEval_pres_Crct in evmch; eauto.
+    destruct i. now eapply Crct_invrt_Construct in evmch as [Hargs _].
+    
+  - intros * evmch IHmch. intros.
+    inv H1.
+    constructor; auto. 
+  - intros. apply H; auto.
+Qed.
+Print Assumptions translate_correct_subst.
